ed25519 derivation: pair programming with jgross... slow progress

src/Specific/Ed25519.v
@@ -14,7 +14,69 @@ Local Arguments H {_} _.
 Local Arguments scalarMultM1 {_} {_} _ _.
 Local Arguments unifiedAddM1 {_} {_} _ _.
 
-Lemma sharper_verify : { verify | forall pk l msg sig, verify pk l msg sig = ed25519_verify pk l msg sig}.
+Ltac set_evars :=
+  repeat match goal with
+         | [ |- appcontext[?E] ] => is_evar E; let e := fresh "e" in set (e := E)
+         end.
+Ltac subst_evars :=
+  repeat match goal with
+         | [ e := ?E |- _ ] => is_evar E; subst e
+         end.
+
+Axiom point_eqb : forall {prm : TwistedEdwardsParams}, point -> point -> bool.
+Axiom point_eqb_correct : forall P Q, point_eqb P Q = if point_eq_dec P Q then true else false.
+
+Require Import Coq.Setoids.Setoid.
+Require Import Coq.Classes.Morphisms.
+Global Instance option_rect_Proper_nd {A T}
+  : Proper ((pointwise_relation _ eq) ==> eq  ==> eq ==> eq) (@option_rect A (fun _ => T)).
+Proof.
+  intros ?? H ??? [|]??; subst; simpl; congruence.
+Qed.
+
+Global Instance option_rect_Proper_nd' {A T}
+  : Proper ((pointwise_relation _ eq) ==> eq  ==> forall_relation (fun _ => eq)) (@option_rect A (fun _ => T)).
+Proof.
+  intros ?? H ??? [|]; subst; simpl; congruence.
+Qed.
+
+Hint Extern 1 (Proper _ (@option_rect ?A (fun _ => ?T))) => exact (@option_rect_Proper_nd' A T) : typeclass_instances.
+
+Lemma option_rect_option_map : forall {A B C} (f:A->B) some none v,
+    option_rect (fun _ => C) (fun x => some (f x)) none v = option_rect (fun _ => C) some none (option_map f v).
+Proof.
+  destruct v; reflexivity.
+Qed.
+
+Axiom decode_scalar : word b -> option N.
+Local Existing Instance Ed25519.FlEncoding.
+Axiom decode_scalar_correct : forall x, decode_scalar x = option_map (fun x : F (Z.of_nat Ed25519.l) => Z.to_N x) (dec x).
+
+Local Infix "==?" := point_eqb (at level 70) : E_scope.
+
+Axiom negate : point -> point.
+Definition point_sub P Q := (P + negate Q)%E.
+Infix "-" := point_sub : E_scope.
+Axiom solve_for_R : forall A B C, (A ==? B + C)%E = (B ==? A - C)%E.
+
+Axiom negateExtended : extendedPoint -> extendedPoint.
+Axiom negateExtended_correct : forall P, negate (unExtendedPoint P) = unExtendedPoint (negateExtended P).
+
+Local Existing Instance PointEncoding.
+Axiom decode_point_eq : forall (P_ Q_ : word (S (b-1))) (P Q:point), dec P_ = Some P -> dec Q_ = Some Q -> weqb P_ Q_ = (P ==? Q)%E.
+
+Lemma decode_test_encode_test : forall S_ X, option_rect (fun _ : option point => bool)
+ (fun S : point => (S ==? X)%E) false (dec S_) = weqb S_ (enc X).
+Proof.
+  intros.
+  destruct (dec S_) eqn:H.
+  { symmetry; eauto using decode_point_eq, encoding_valid. }
+  { simpl @option_rect.
+    destruct (weqb S_ (enc X)) eqn:Heqb; trivial.
+    apply weqb_true_iff in Heqb. subst. rewrite encoding_valid in H; discriminate. }
+Qed.
+
+Lemma sharper_verify : forall pk l msg sig, { verify | verify = ed25519_verify pk l msg sig}.
 Proof.
   eexists; intros.
   cbv [ed25519_verify EdDSA.verify
@@ -22,28 +84,72 @@ Proof.
                       EdDSA.E EdDSA.B EdDSA.b EdDSA.l EdDSA.H
                       EdDSA.PointEncoding EdDSA.FlEncoding EdDSA.FqEncoding].
 
-  (* zoom in to the interesting case *)
-  repeat match goal with |- context[match ?a with Some x => _ | _ => _ end] =>
-                    let n := fresh x in
-                    let H := fresh "Heq" x in
-                    destruct a as [x|]
-  end.
+  etransitivity.
+  Focus 2.
+  { repeat match goal with
+           | [ |- ?x = ?x ] => reflexivity
+           | [ |- _ = match ?a with None => ?N | Some x => @?S x end :> ?T ]
+             => etransitivity;
+               [
+               | refine (_ : option_rect (fun _ => T) _ N a = _);
+                 let S' := match goal with |- option_rect _ ?S' _ _ = _ => S' end in
+                 refine (option_rect (fun a' => option_rect (fun _ => T) S' N a' = match a' with None => N | Some x => S x end)
+                                     (fun x => _) _ a); intros; simpl @option_rect ];
+               [ reflexivity | .. ]
+           end.
+    set_evars.
+    rewrite<- point_eqb_correct.
+    rename x0 into R. rename x1 into S. rename x into A.
+    rewrite solve_for_R.
+    let p1 := constr:(scalarMultM1_rep eq_refl) in
+    let p2 := constr:(unifiedAddM1_rep eq_refl) in
+    repeat match goal with
+           | |- context [(_ * ?P)%E] =>
+              rewrite <-(unExtendedPoint_mkExtendedPoint P);
+               rewrite <-p1
+           | |- context [(?P + unExtendedPoint _)%E] =>
+             rewrite <-(unExtendedPoint_mkExtendedPoint P);
+               rewrite p2
+           end;
+      rewrite ?Znat.Z_nat_N, <-?Word.wordToN_nat;
+      subst_evars;
+      reflexivity.
+    } Unfocus.
 
-  let p1 := constr:(scalarMultM1_rep eq_refl) in
-  let p2 := constr:(unifiedAddM1_rep eq_refl) in
-  repeat match goal with
-  | |- context [(?n * ?P)%E] =>
-    rewrite <-(unExtendedPoint_mkExtendedPoint P);
-    erewrite <-p1
-  | |- context [(?P + unExtendedPoint _)%E] =>
-    rewrite <-(unExtendedPoint_mkExtendedPoint P);
-    erewrite p2
-  end.
-  rewrite !Znat.Z_nat_N, <-!Word.wordToN_nat.
-  
+  etransitivity.
+  Focus 2.
+  { lazymatch goal with |- _ = option_rect _ _ ?false ?dec =>
+                    symmetry; etransitivity; [|eapply (option_rect_option_map (fun (x:F _) => Z.to_N x) _ false dec)]
+    end.
+    eapply option_rect_Proper_nd; [intro|reflexivity..].
+    match goal with
+    | [ |- ?RHS = ?e ?v ]
+      => let RHS' := (match eval pattern v in RHS with ?RHS' _ => RHS' end) in
+        unify e RHS'
+    end.
+    reflexivity.
+  } Unfocus.
+  rewrite <-decode_scalar_correct.
+
+  etransitivity.
+  Focus 2.
+  { do 2 (eapply option_rect_Proper_nd; [intro|reflexivity..]).
+    symmetry; apply decode_test_encode_test.
+  } Unfocus.
+
+  etransitivity.
+  Focus 2.
+  { do 2 (eapply option_rect_Proper_nd; [intro|reflexivity..]).
+    unfold point_sub. rewrite negateExtended_correct.
+    let p := constr:(unifiedAddM1_rep eq_refl) in rewrite p.
+    reflexivity.
+  } Unfocus.
+
   cbv [scalarMultM1 iter_op].
-  Local Arguments funexp {_} _ {_} {_}. (* do not display the initializer and iteration bound for now *)
   cbv iota zeta delta [test_and_op].
+  Local Arguments funexp {_} _ {_} {_}. (* do not display the initializer and iteration bound for now *)
 
-
+  Axiom rep : forall {m}, list Z -> F m -> Prop.
+  Axiom decode_point_limbs : word (S (b-1)) -> option (list Z * list Z).
+  Axiom point_dec_rep : forall P_ P lx ly, dec P_ = Some P -> decode_point_limbs P_ = Some (lx, ly) -> rep lx (fst (proj1_sig P)) /\ rep ly (fst (proj1_sig P)).
 Admitted.
